specs/lib/Spec.Lib.IntSeq.fsti
@@ -62,4 +62,4 @@ val uint_from_bytes_be: #t:inttype -> intseq U8 (numbytes t) -> u:uint_t t
 val uints_to_bytes_le: #t:inttype -> #len:size_t{len `op_Multiply` numbytes t < pow2 32} -> intseq t len -> lbytes (len `op_Multiply` numbytes t)
 val uints_to_bytes_be: #t:inttype -> #len:size_t{len `op_Multiply` numbytes t < pow2 32} -> intseq t len -> lbytes (len `op_Multiply` numbytes t)
 val uints_from_bytes_le: #t:inttype -> #len:size_t{len `op_Multiply` numbytes t < pow2 32} -> lbytes (len `op_Multiply` numbytes t) -> intseq t len
-val uints_from_bytes_be: #t:inttype -> #len:size_t{len `op_Multiply` numbytes t < pow2 32} -> lbytes (len `op_Multiply` numbytes t) -> intseq t len
+  val uints_from_bytes_be: #t:inttype -> #len:size_t{len `op_Multiply` numbytes t < pow2 32} -> lbytes (len `op_Multiply` numbytes t) -> intseq t len
